thys/Untyped_Lambda_Calculus/LC_Beta.thy
@@ -5,20 +5,20 @@ imports LC "Binders.Generic_Barendregt_Enhanced_Rule_Induction" "Prelim.Curry_LF
 begin
 
 inductive step :: "trm \<Rightarrow> trm \<Rightarrow> bool" where
-  Beta: "step (App (Lam x e1) e2) (tvsubst (Var(x:=e2)) e1)"
-| AppL: "step e1 e1' \<Longrightarrow> step (App e1 e2) (App e1' e2)"
-| AppR: "step e2 e2' \<Longrightarrow> step (App e1 e2) (App e1 e2')"
-| Xi: "step e e' \<Longrightarrow> step (Lam x e) (Lam x e')"
+  Beta: "step (Ap (Lm x e1) e2) (tvsubst (Vr(x:=e2)) e1)"
+| AppL: "step e1 e1' \<Longrightarrow> step (Ap e1 e2) (Ap e1' e2)"
+| AppR: "step e2 e2' \<Longrightarrow> step (Ap e1 e2) (Ap e1 e2')"
+| Xi: "step e e' \<Longrightarrow> step (Lm x e) (Lm x e')"
 
 binder_inductive step
   subgoal premises prems for R B t1 t2  \<comment> \<open>refreshability\<close>
     by (tactic \<open>refreshability_tac false
-      [@{term "FFVars :: trm \<Rightarrow> var set"}, @{term "FFVars :: trm \<Rightarrow> var set"}]
+      [@{term "FV :: trm \<Rightarrow> var set"}, @{term "FV :: trm \<Rightarrow> var set"}]
       [@{term "rrename :: (var \<Rightarrow> var) \<Rightarrow> trm \<Rightarrow> trm"}, @{term "(\<lambda>f x. f x) :: (var \<Rightarrow> var) \<Rightarrow> var \<Rightarrow> var"}]
       [SOME [SOME 1, SOME 0, NONE], NONE, NONE, SOME [SOME 0, SOME 0, SOME 1]]
       @{thm prems(3)} @{thm prems(2)} @{thms }
       @{thms emp_bound singl_bound term.Un_bound term.set_bd_UNIV infinite}
-      @{thms Lam_inject} @{thms Lam_eq_tvsubst term.permute_cong_id[symmetric]}
+      @{thms Lm_inject} @{thms Lm_eq_tvsubst term.permute_cong_id[symmetric]}
       @{thms } @{context}\<close>)
   done
 
