thys/Untyped_Lambda_Calculus/LC_Parallel_Beta.thy
@@ -6,19 +6,19 @@ begin
 
 inductive pstep :: "trm \<Rightarrow> trm \<Rightarrow> bool" where
   Refl: "pstep e e"
-| App: "pstep e1 e1' \<Longrightarrow> pstep e2 e2' \<Longrightarrow> pstep (App e1 e2) (App e1' e2')"
-| Xi: "pstep e e' \<Longrightarrow> pstep (Lam x e) (Lam x e')"
-| PBeta: "pstep e1 e1' \<Longrightarrow> pstep e2 e2' \<Longrightarrow> pstep (App (Lam x e1) e2) (tvsubst (Var(x:=e2')) e1')"
+| Ap: "pstep e1 e1' \<Longrightarrow> pstep e2 e2' \<Longrightarrow> pstep (Ap e1 e2) (Ap e1' e2')"
+| Xi: "pstep e e' \<Longrightarrow> pstep (Lm x e) (Lm x e')"
+| PBeta: "pstep e1 e1' \<Longrightarrow> pstep e2 e2' \<Longrightarrow> pstep (Ap (Lm x e1) e2) (tvsubst (Vr(x:=e2')) e1')"
 
 binder_inductive pstep
   subgoal premises prems for R B t1 t2
     by (tactic \<open>refreshability_tac false
-      [@{term "FFVars :: trm \<Rightarrow> var set"}, @{term "FFVars :: trm \<Rightarrow> var set"}]
+      [@{term "FV :: trm \<Rightarrow> var set"}, @{term "FV :: trm \<Rightarrow> var set"}]
       [@{term "rrename :: (var \<Rightarrow> var) \<Rightarrow> trm \<Rightarrow> trm"}, @{term "(\<lambda>f x. f x) :: (var \<Rightarrow> var) \<Rightarrow> var \<Rightarrow> var"}]
       [NONE, NONE, SOME [SOME 0, SOME 0, SOME 1], SOME [SOME 0, SOME 0, NONE, NONE, SOME 1]]
       @{thm prems(3)} @{thm prems(2)} @{thms }
       @{thms emp_bound singl_bound term.Un_bound term.set_bd_UNIV infinite}
-      @{thms Lam_inject} @{thms Lam_eq_tvsubst term.permute_cong_id[symmetric]}
+      @{thms Lm_inject} @{thms Lm_eq_tvsubst term.permute_cong_id[symmetric]}
       @{thms id_on_antimono} @{context}\<close>)
   done
 
